CleanQ/CleanQ_RBModel.thy
@@ -1339,11 +1339,11 @@ definition CleanQ_RB_enq_y_pre :: "'a set \<Rightarrow> 'a \<Rightarrow> ('a Cle
   where "CleanQ_RB_enq_y_pre K b = Semantic.Normal ` {rb. CleanQ_RB_Invariants K rb \<and> CleanQ_RB_enq_y_possible rb \<and> b \<in> rSY rb}"
 
 definition CleanQ_RB_deq_x_pre :: "'a set \<Rightarrow> 'a \<Rightarrow> ('a CleanQ_RB_State, 'a CleanQ_RB_State) Semantic.xstate set"        
-  where "CleanQ_RB_deq_x_pre K buf = Semantic.Normal ` {rb. I1_rb_img rb K \<and> I2_rb_img rb \<and> I3_rb_img rb \<and>
-                                                        CleanQ_RB_list  (rTYX rb) \<noteq> [] \<and> buf = ring (rTYX rb) (tail (rTYX rb))}"
+  where "CleanQ_RB_deq_x_pre K buf = Semantic.Normal ` {rb. CleanQ_RB_Invariants K rb \<and> CleanQ_RB_deq_x_possible rb \<and>
+                                                        buf = ring (rTYX rb) (tail (rTYX rb))}"
 definition CleanQ_RB_deq_y_pre :: "'a set \<Rightarrow> 'a \<Rightarrow> ('a CleanQ_RB_State, 'a CleanQ_RB_State) Semantic.xstate set"        
-  where "CleanQ_RB_deq_y_pre K buf = Semantic.Normal ` {rb. I1_rb_img rb K \<and> I2_rb_img rb \<and> I3_rb_img rb \<and>
-                                                        CleanQ_RB_list  (rTXY rb) \<noteq> [] \<and> buf = ring (rTXY rb) (tail (rTXY rb))}"
+  where "CleanQ_RB_deq_y_pre K buf = Semantic.Normal ` {rb. CleanQ_RB_Invariants K rb \<and> CleanQ_RB_deq_y_possible rb \<and>
+                                                        buf = ring (rTXY rb) (tail (rTXY rb))}"
 
 
   
