CleanQ/CleanQ_ListRBRefinement.thy
@@ -18,6 +18,8 @@ theory CleanQ_ListRBRefinement imports
   CleanQ_RBModel
 begin
 
+declare [[ smt_timeout = 120 ]]
+
 lemma
   CleanQ_listRBRefinement_enq_x: 
   assumes precond: "Semantic.xstate.Normal sc \<in> CleanQ_RB_enq_x_pre K buf" 
@@ -60,7 +62,7 @@ lemma
   CleanQ_listRBRefinement_enq_y: 
   assumes precond: "Semantic.xstate.Normal sc \<in> CleanQ_RB_enq_y_pre K buf" 
   shows
-  "((\<Gamma>a, CleanQ_List_enq_x_pre K buf, Language.Basic (CleanQ_List_enq_y buf)), 
+  "((\<Gamma>a, CleanQ_List_enq_y_pre K buf, Language.Basic (CleanQ_List_enq_y buf)), 
                                (\<Gamma>c, CleanQ_RB_enq_y_pre K buf, Language.Basic (CleanQ_RB_enq_y buf)))
                                \<in> refinement_s (separable_lift CleanQ_RB2List CleanQ_RB2List)"
   apply(rule refinement_s_BasicI) (* Problem applying this after unfolding*)
@@ -88,19 +90,63 @@ proof -
    show "Semantic.xstate.case_xstate (\<lambda>sc. Semantic.xstate.Normal (CleanQ_RB2List sc)) (\<lambda>sc. Abrupt (CleanQ_RB2List sc)) (\<lambda>fc. Semantic.xstate.Fault (CleanQ_RB2List fc))
      Semantic.xstate.Stuck ` CleanQ_RB_enq_y_pre K buf \<subseteq> CleanQ_List_enq_y_pre K buf"
      using core_g2 CleanQ_RB_Invariants_List_Invariants unfolding CleanQ_RB_enq_y_pre_def CleanQ_List_enq_y_pre_def
-     try
+     by (smt CleanQ_List_State.select_convs(2) CleanQ_List_State.select_convs(4) CleanQ_RB2List_def CleanQ_RB_Invariants.elims(2) I2_rb_img.elims(2)
+         Semantic.xstate.simps(16) disjoint_iff_not_equal image_Collect_subsetI image_def mem_Collect_eq)
 qed
 
+lemma 
+  refine_hd_list_tl_ring:
+  fixes buf sc
+  assumes precond: "Semantic.xstate.Normal sc \<in> CleanQ_RB_deq_x_pre K buf"
+  shows "buf = ring (rTYX sc) (tail (rTYX sc)) \<Longrightarrow> buf = hd (lTYX (CleanQ_RB2List sc))"
+  unfolding CleanQ_RB2List_def using precond 
+  apply auto
+  by (metis (mono_tags, lifting) CleanQ_RB_Invariants.elims(2) CleanQ_RB_deq_x_possible_def CleanQ_RB_deq_x_pre_def 
+      CollectD I4_rb_valid.elims(2) imageE prod.sel(1) rb_deq_def rb_deq_list_was_head state_simps(1))   
 
 lemma
-  CleanQ_listRBRefinement_deq_x: "((\<Gamma>a, CleanQ_List_deq_x_pre K buf, Language.Basic (CleanQ_List_deq_x)), 
-                               (\<Gamma>c, CleanQ_RB_deq_x_pre K buf, Language.Basic (CleanQ_RB_deq_x)))
+  CleanQ_listRBRefinement_deq_x:   
+  assumes precond: "Semantic.xstate.Normal sc \<in> CleanQ_RB_deq_x_pre K buf" 
+  shows
+  "((\<Gamma>a, CleanQ_List_deq_x_pre K buf, Language.Basic (CleanQ_List_deq_x)), 
+    (\<Gamma>c, CleanQ_RB_deq_x_pre K buf, Language.Basic (CleanQ_RB_deq_x)))
                                \<in> refinement_s (separable_lift CleanQ_RB2List CleanQ_RB2List)"
   apply(rule refinement_s_BasicI) (* Problem applying this after unfolding*)
-    unfolding separable_lift_def  CleanQ_List_deq_x_def CleanQ_List_deq_x_pre_def CleanQ_RB_deq_x_def
-   CleanQ_RB_deq_x_pre_def
-  proof(auto)
-    oops
+  unfolding separable_lift_def
+proof -
+    show "\<And>sc. Semantic.xstate.Normal sc \<in> CleanQ_RB_deq_x_pre K buf \<Longrightarrow> CleanQ_RB2List (CleanQ_RB_deq_x sc) = CleanQ_List_deq_x (CleanQ_RB2List sc)" 
+    using CleanQ_RB_deq_x_equal
+    by (smt CleanQ_RB_deq_x_pre_def CollectD image_def state_simps(1))
+next
+   fix b
+   have b_in_tyx: "b \<in> set (CleanQ_RB_list (rTYX sc)) \<Longrightarrow> b \<in> set (lTYX (CleanQ_RB2List sc))"
+      by (simp add: CleanQ_RB2List_def)
+   have b_notin_sx: "b \<in> set (CleanQ_RB_list (rTYX sc)) \<Longrightarrow> b \<notin> (lSX (CleanQ_RB2List sc))" 
+     using precond
+     unfolding CleanQ_RB_deq_x_pre_def CleanQ_RB2List_def
+     by auto
+   have non_empty: "CleanQ_RB_deq_x_possible sc \<Longrightarrow> lTYX (CleanQ_RB2List sc) \<noteq> []" 
+     using precond unfolding CleanQ_RB_deq_x_possible_def
+   by (metis (no_types, lifting) CleanQ_List_State.select_convs(4) CleanQ_RB2List_def 
+      CleanQ_RB_Invariants.elims(2) CleanQ_RB_deq_x_pre_def CollectD I3_rb_img.elims(2) 
+      I4_rb_valid.elims(2) image_iff list.sel(2) rb_deq_list_not_in rb_deq_list_tail rb_deq_list_was_in state_simps(1))
+   have core_g2: "Semantic.xstate.Normal (CleanQ_RB2List sc) \<in> CleanQ_List_deq_x_pre K buf" using precond
+   proof -
+     have precond_buf: " buf = hd (lTYX (CleanQ_RB2List sc)) \<longleftrightarrow> buf = ring (rTYX sc) (tail (rTYX sc))"
+       using precond refine_hd_list_tl_ring
+       by (smt CleanQ_RB_deq_x_pre_def CollectD imageE state_simps(1))
+
+     have final: "Semantic.xstate.Normal sc \<in> CleanQ_RB_deq_x_pre K buf \<Longrightarrow> Semantic.xstate.Normal (CleanQ_RB2List sc) \<in> CleanQ_List_deq_x_pre K buf" 
+       using b_in_tyx b_notin_sx precond non_empty refine_hd_list_tl_ring precond_buf unfolding CleanQ_RB2List_def CleanQ_RB_deq_x_pre_def CleanQ_List_deq_x_pre_def
+       by force
+     show ?thesis using final precond
+       by simp
+   qed
+   show "Semantic.xstate.case_xstate (\<lambda>sc. Semantic.xstate.Normal (CleanQ_RB2List sc)) (\<lambda>sc. Abrupt (CleanQ_RB2List sc)) 
+         (\<lambda>fc. Semantic.xstate.Fault (CleanQ_RB2List fc)) Semantic.xstate.Stuck ` CleanQ_RB_deq_x_pre K buf \<subseteq> CleanQ_List_deq_x_pre K buf"
+     using core_g2 CleanQ_RB_Invariants_List_Invariants refine_hd_list_tl_ring non_empty
+     unfolding CleanQ_RB_deq_x_pre_def CleanQ_List_deq_x_pre_def rb_empty_def
+     sorry
  
 lemma
   CleanQ_listRBRefinement_deq_y: "((\<Gamma>a, CleanQ_List_deq_y_pre K buf, Language.Basic (CleanQ_List_deq_y)), 
